erasure/theories/EWcbvEval.v
@@ -1,7 +1,8 @@
 (* Distributed under the terms of the MIT license.   *)
 Set Warnings "-notation-overridden".
 
-From Coq Require Import Bool List Program.
+From Coq Require Import Arith Bool List Program.
+From Equations Require Import Equations.
 From MetaCoq.Template Require Import config utils.
 From MetaCoq.Erasure Require Import EAst EAstUtils ELiftSubst ECSubst ETyping.
 
@@ -40,23 +41,6 @@ Definition isFixApp t :=
   | _ => false
   end.
 
-Definition isStuckFix t args :=
-  match t with
-  | tFix mfix idx =>
-    match unfold_fix mfix idx with
-    | Some (narg, fn) =>
-      ~~ is_constructor_or_box narg args
-    | None => false
-    end
-  | _ => false
-  end.
-
-Lemma atom_mkApps f l : atom (mkApps f l) -> (l = []) /\ atom f.
-Proof.
-  revert f; induction l using rev_ind. simpl. intuition auto.
-  simpl. intros. now rewrite mkApps_app in H.
-Qed.
-
 Definition substl defs body : term :=
   fold_left (fun bod term => csubst term 0 bod)
     defs body.
@@ -67,6 +51,23 @@ Definition cunfold_fix (mfix : mfixpoint term) (idx : nat) :=
     Some (d.(rarg), substl (fix_subst mfix) d.(dbody))
   | None => None
   end.
+
+Definition isStuckFix t args :=
+  match t with
+  | tFix mfix idx =>
+    match cunfold_fix mfix idx with
+    | Some (narg, fn) =>
+      ~~ is_nth_constructor_app_or_box narg args
+    | None => false
+    end
+  | _ => false
+  end.
+
+Lemma atom_mkApps f l : atom (mkApps f l) -> (l = []) /\ atom f.
+Proof.
+  revert f; induction l using rev_ind. simpl. intuition auto.
+  simpl. intros. now rewrite mkApps_app in H.
+Qed.
 
 Definition cunfold_cofix (mfix : mfixpoint term) (idx : nat) :=
   match List.nth_error mfix idx with
@@ -112,29 +113,23 @@ Section Wcbv.
       eval (mkApps f (repeat tBox n)) res ->
       eval (tCase (ind, pars) discr brs) res
 
-  (** Fix unfolding *)
-  | eval_fix f mfix idx args args' narg fn res :
-      eval f (tFix mfix idx) ->
+  (** Fix unfolding, with guard *)
+  | eval_fix f mfix idx argsv a av narg fn res :
+      eval f (mkApps (tFix mfix idx) argsv) ->
+      eval a av ->
       cunfold_fix mfix idx = Some (narg, fn) ->
-      (* There must be at least one argument for this to succeed *)
-      is_constructor_or_box narg args' ->
-      (** We unfold only a fix applied exactly to narg arguments,
-          avoiding overlap with [eval_beta] when there are more arguments. *)
-      S narg = #|args| ->
-      (* We reduce all arguments before unfolding *)
-      Forall2 eval args args' ->
-      eval (mkApps fn args') res ->
-      eval (mkApps f args) res
+      #|argsv| = narg ->
+      is_constructor_app_or_box av ->
+      eval (tApp (mkApps fn argsv) av) res ->
+      eval (tApp f a) res
 
-  (** Fix stuck *)
-  | eval_fix_value f mfix idx args args' :
-      eval f (tFix mfix idx) ->
-      (* We reduce all arguments to produce a suspended fix application value
-         Note that the stuck fixpoint can be applied to any number of arguments
-         here. *)
-      Forall2 eval args args' ->
-      isStuckFix (tFix mfix idx) args' ->
-      eval (mkApps f args) (mkApps (tFix mfix idx) args')
+  (** Fix stuck, with guard *)
+  | eval_fix_value f mfix idx argsv a av narg fn :
+      eval f (mkApps (tFix mfix idx) argsv) ->
+      eval a av ->
+      cunfold_fix mfix idx = Some (narg, fn) ->
+      (#|argsv| <> narg \/ (#|argsv| = narg /\ ~~is_constructor_app_or_box av)) ->
+      eval (tApp f a) (tApp (mkApps (tFix mfix idx) argsv) av)
 
   (** CoFix-case unfolding *)
   | red_cofix_case ip mfix idx args narg fn brs res :
@@ -183,87 +178,8 @@ Section Wcbv.
   | eval_atom t : atom t -> eval t t.
 
   Hint Constructors eval : core.
-
-  (* Scheme Minimality for eval Sort Type. *)
-  Definition eval_evals_ind :
-    forall P : term -> term -> Prop,
-      (forall a t t', eval a tBox -> P a tBox -> eval t t' -> P t t' -> eval (tApp a t) tBox -> P (tApp a t) tBox ) ->
-      (forall (f : term) (na : name) (b a a' res : term),
-          eval f (tLambda na b) ->
-          P f (tLambda na b) -> eval a a' -> P a a' -> eval (csubst a' 0 b) res -> P (csubst a' 0 b) res -> P (tApp f a) res) ->
-      (forall (na : name) (b0 b0' b1 res : term),
-          eval b0 b0' -> P b0 b0' -> eval (csubst b0' 0 b1) res -> P (csubst b0' 0 b1) res -> P (tLetIn na b0 b1) res) ->
-      (forall c (decl : constant_body) (body : term),
-          declared_constant Σ c decl ->
-          forall (res : term),
-            cst_body decl = Some body ->
-            eval body res -> P body res -> P (tConst c) res) ->
-      (forall (ind : inductive) (pars : nat) (discr : term) (c : nat)
-              (args : list term) (brs : list (nat × term)) (res : term),
-          eval discr (mkApps (tConstruct ind c) args) ->
-          P discr (mkApps (tConstruct ind c) args) ->
-          eval (iota_red pars c args brs) res -> P (iota_red pars c args brs) res -> P (tCase (ind, pars) discr brs) res) ->
-      (forall ind pars discr brs n f res,
-          eval discr tBox -> P discr tBox ->
-          brs = [(n, f)] ->
-          eval (mkApps f (repeat tBox n)) res -> P (mkApps f (repeat tBox n)) res ->
-          eval (tCase (ind, pars) discr brs) res -> P (tCase (ind, pars) discr brs) res
-      ) ->
-      (forall (i : inductive) (pars arg : nat) (discr : term) (args : list term) (k : nat)
-              (a res : term),
-          eval discr (mkApps (tConstruct i k) args) ->
-          P discr (mkApps (tConstruct i k) args) ->
-          eval (nth (pars + arg) args tDummy) res -> P (nth (pars + arg) args tDummy) res -> P (tProj (i, pars, arg) discr) res) ->
-      (forall i pars arg discr,
-          eval discr tBox -> P discr tBox ->
-          eval (tProj (i, pars, arg) discr) tBox -> P (tProj (i, pars, arg) discr) tBox
-      ) ->
-      (forall f (mfix : mfixpoint term) (idx : nat) (args args' : list term) (narg : nat) (fn res : term),
-          eval f (tFix mfix idx) ->
-          P f (tFix mfix idx) ->
-          cunfold_fix mfix idx = Some (narg, fn) ->
-          is_constructor_or_box narg args' ->
-          S narg = #|args| ->
-          Forall2 eval args args' ->
-          Forall2 P args args' ->
-          eval (mkApps fn args') res -> P (mkApps fn args') res -> P (mkApps f args) res) ->
-      (forall f (mfix : mfixpoint term) (idx : nat) (args args' : list term),
-          eval f (tFix mfix idx) ->
-          P f (tFix mfix idx) ->
-          Forall2 eval args args' ->
-          Forall2 P args args' ->
-          isStuckFix (tFix mfix idx) args' -> P (mkApps f args) (mkApps (tFix mfix idx) args')) ->
-      (forall (ip : inductive × nat) (mfix : mfixpoint term) (idx : nat) (args : list term)
-              (narg : nat) (fn : term) (brs : list (nat × term)) (res : term),
-          cunfold_cofix mfix idx = Some (narg, fn) ->
-          eval (tCase ip (mkApps fn args) brs) res ->
-          P (tCase ip (mkApps fn args) brs) res -> P (tCase ip (mkApps (tCoFix mfix idx) args) brs) res) ->
-      (forall (p : projection) (mfix : mfixpoint term) (idx : nat) (args : list term) (narg : nat) (fn res : term),
-          cunfold_cofix mfix idx = Some (narg, fn) ->
-          eval (tProj p (mkApps fn args)) res ->
-          P (tProj p (mkApps fn args)) res -> P (tProj p (mkApps (tCoFix mfix idx) args)) res) ->
-      (forall f11 f' a a' : term,
-          eval f11 f' -> P f11 f' -> ~~ (isLambda f' || isFixApp f' || isBox f') -> eval a a' -> P a a' -> P (tApp f11 a) (tApp f' a')) ->
-      (forall t : term, atom t -> P t t) -> forall t t0 : term, eval t t0 -> P t t0.
-  Proof.
-    intros P Hbox Hbeta Hlet Hcst Hcase Hsing Hproj Hprojbox Hfix Hstuckfix Hcofixcase Hcofixproj Happcong Hatom.
-    fix eval_evals_ind 3. destruct 1;
-             try solve [match goal with [ H : _ |- _ ] =>
-                             match type of H with
-                               forall t t0, eval t t0 -> _ => fail 1
-                             | _ => eapply H
-                             end end; eauto].
-    - eapply Hbox; eauto.
-    - eapply Hcase; eauto.
-    - eapply Hfix; eauto.
-      clear -H3 eval_evals_ind.
-      revert args args' H3. fix aux 3. destruct 1. constructor; auto.
-      constructor. now apply eval_evals_ind. now apply aux.
-    - eapply Hstuckfix => //. eapply eval_evals_ind. auto.
-      clear -eval_evals_ind H0.
-      revert args args' H0. fix aux 3. destruct 1. constructor; auto.
-      constructor. now apply eval_evals_ind. now apply aux.
-  Qed.
+  Derive Signature for eval.
+  Derive NoConfusionHom for term.
 
   (** Characterization of values for this reduction relation.
       Only constructors and cofixpoints can accumulate arguments.
@@ -360,22 +276,46 @@ Section Wcbv.
 
   Lemma eval_to_value e e' : eval e e' -> value e'.
   Proof.
-    induction 1 using eval_evals_ind; simpl; auto using value.
-    (* eapply (value_app (tEvar n l') []). constructor. constructor. *)
-    - eapply value_stuck_fix => //.
-      now eapply Forall2_right in H1.
+    induction 1; simpl; auto using value.
+    - change (tApp ?h ?a) with (mkApps h [a]).
+      rewrite mkApps_nested.
+      apply value_mkApps_inv in IHeval1; [|easy].
+      destruct IHeval1 as [(-> & _)|[|(stuck & vals)]].
+      + cbn in *.
+        apply (value_stuck_fix _ [av]); [easy|].
+        cbn.
+        destruct (cunfold_fix mfix idx) as [(? & ?)|]; [|easy].
+        noconf H1.
+        destruct H2 as [|(<- & ?)]; [|easy].
+        unfold is_nth_constructor_app_or_box.
+        now rewrite (proj2 (nth_error_None _ _));
+          cbn in *.
+      + easy.
+      + eapply value_stuck_fix; [now apply Forall_app_inv|].
+        unfold isStuckFix in *.
+        destruct (cunfold_fix mfix idx) as [(? & ?)|]; [|easy].
+        noconf H1.
+        unfold is_nth_constructor_app_or_box in *.
+        destruct H2 as [|(<- & ?)]; [|now rewrite nth_error_snoc].
+        destruct (Nat.ltb_spec #|argsv| narg).
+        * rewrite (proj2 (nth_error_None _ _)); [|easy].
+          rewrite app_length.
+          cbn.
+          easy.
+        * now rewrite nth_error_app1.
+
     - destruct (mkApps_elim f' [a']).
       eapply value_mkApps_inv in IHeval1 => //.
       destruct IHeval1; intuition subst.
       * rewrite H3.
         simpl. rewrite H3 in H. simpl in *.
-        apply (value_app f [a']). rewrite H3 in H0. destruct f; simpl in * |- *; try congruence.
+        apply (value_app f0 [a']). rewrite H3 in H0. destruct f0; simpl in * |- *; try congruence.
         constructor; auto. constructor. constructor; auto.
       * rewrite [tApp _ _](mkApps_nested _ (firstn n l) [a']).
         constructor 2; auto. eapply Forall_app_inv; auto.
       * rewrite [tApp _ _](mkApps_nested _ (firstn n l) [a']).
         erewrite isFixApp_mkApps in H0 => //.
-        destruct f; simpl in *; try congruence.
+        destruct f0; simpl in *; try congruence.
         rewrite /isFixApp in H0. simpl in H0.
         rewrite orb_true_r orb_true_l in H0. easy.
   Qed.
@@ -430,247 +370,176 @@ Section Wcbv.
     f_equal. rewrite lift_closed // closed_subst //.
   Qed.
 
+Lemma eval_mkApps_tCoFix mfix idx args v :
+  eval (mkApps (tCoFix mfix idx) args) v ->
+  exists args', v = mkApps (tCoFix mfix idx) args'.
+Proof.
+  revert v.
+  induction args using List.rev_ind; intros v ev.
+  + exists [].
+    now depelim ev.
+  + rewrite mkApps_app in ev.
+    cbn in *.
+    depelim ev;
+      try (apply IHargs in ev1 as (? & ?); solve_discr).
+    * apply IHargs in ev1 as (argsv & ->).
+      exists (argsv ++ [a']).
+      now rewrite mkApps_app.
+    * easy.
+Qed.
 
-  (* Lemma eval_to_value e e' : eval e e' -> value e'. *)
-  (* Proof. *)
-  (*   induction 1 using eval_ind; simpl; auto using value. *)
-  (*   - eapply value_stuck_fix => //. *)
+Derive NoConfusionHom for EAst.global_decl.
 
-  (*     eapply Forall2_right. *)
-  (*     eauto. *)
-  (*     admit. *)
-  (*   - destruct (mkApps_elim f' [a']). *)
-  (*     eapply value_mkApps_inv in IHeval1 => //. *)
-  (*     destruct IHeval1; intuition subst. *)
-  (*     * rewrite H3. *)
-  (*       simpl. rewrite H3 in H. simpl in *. *)
-  (*       apply (value_app f0 [a']). destruct f0; simpl in * |- *; try congruence. *)
-
-  (*       constructor; auto. constructor. constructor; auto. *)
-  (*     * rewrite [tApp _ _](mkApps_nested _ (firstn n l) [a']). *)
-  (*       constructor 2; auto. eapply All_app_inv; auto. *)
-  (*     * rewrite [tApp _ _](mkApps_nested _ (firstn n l) [a']). *)
-  (*       rewrite isFixApp_mkApps in H => //. *)
-  (*       destruct f; simpl in *; try congruence. *)
-  (*       rewrite /isFixApp in H. simpl in H. *)
-  (*       rewrite orb_true_r orb_true_l in H. easy. *)
-  (* Qed. *)
-  (* Admitted. *)
-
-  (* Lemma value_final e : value e -> eval e e. *)
-  (* Proof. *)
-  (*   induction 1 using value_values_ind; simpl; auto using value. *)
-  (*   now constructor. *)
-  (*   assert (Forall2 eval l l). *)
-  (*   induction H1; constructor; auto. eapply IHForall. now depelim H0. *)
-  (*   rewrite value_head_spec in H. *)
-  (*   induction l using rev_ind. simpl. *)
-  (*   move/andP: H => [H H']. *)
-  (*   constructor; try easy. *)
-  (*   rewrite mkApps_app. *)
-  (*   eapply Forall_app in H0 as [Hl Hx]. depelim Hx. *)
-  (*   eapply Forall2_app_r in H2 as [Hl' Hx']. *)
-  (*   eapply eval_app_cong; auto. *)
-  (*   eapply IHl. auto. *)
-  (*   now eapply Forall2_Forall. auto. *)
-  (*   move/andP: H => [Ht Ht']. *)
-  (*   destruct l using rev_ind; auto. now rewrite mkApps_app; simpl. *)
-  (* Qed. *)
-
-  (* (** Evaluation preserves closedness: *) *)
-  (* Lemma eval_closed : forall n t u, closedn n t = true -> eval t u -> closedn n u = true. *)
-  (* Proof. *)
-  (*   induction 2 using eval_ind; simpl in *; auto. eapply IHeval3. *)
-  (*   admit. *)
-  (* Admitted. (* closedness of evaluates for Eterms, not needed for verification *) *)
-
-  (* Lemma eval_tApp_tFix_inv mfix idx a v : *)
-  (*   eval (tApp (tFix mfix idx) a) v -> *)
-  (*   (exists fn arg, *)
-  (*       (unfold_fix mfix idx = Some (arg, fn)) /\ *)
-  (*       (eval (tApp fn a) v)). *)
-  (* Proof. *)
-  (*   intros H; depind H; try solve_discr. *)
-  (*   - depelim H. *)
-  (*   - depelim H. *)
-  (*   - eexists _, _; firstorder eauto.  *)
-  (*   - now depelim H. *)
-  (*   - discriminate. *)
-  (* Qed. *)
-
-  (* Lemma eval_tBox t : eval tBox t -> t = tBox. *)
-  (* Proof. *)
-  (*   intros H; depind H; try solve_discr. auto. *)
-  (* Qed. *)
-
-  (* Lemma eval_tRel n t : eval (tRel n) t -> False. *)
-  (* Proof. *)
-  (*   intros H; depind H; try solve_discr; try now easy. *)
-  (* Qed. *)
-
-  (* Lemma eval_tVar i t : eval (tVar i) t -> False. *)
-  (* Proof. *)
-  (*   intros H; depind H; try solve_discr; try now easy. *)
-  (* Qed. *)
-
-  (* Lemma eval_tEvar n l t : eval (tEvar n l) t -> False. *)
-  (*                         (* exists l', Forall2 eval l l' /\ (t = tEvar n l'). *) *)
-  (* Proof. *)
-  (*   intros H; depind H; try solve_discr; try now easy. *)
-  (* Qed. *)
-
-  (* (* Lemma eval_atom_inj t t' : atom t -> eval t t' -> t = t'. *) *)
-  (* (* Proof. *) *)
-  (* (*   intros Ha H; depind H; try solve_discr; try now easy. *) *)
-  (* (* Qed. *) *)
-
-  (* Lemma eval_LetIn {n b t v} : *)
-  (*   eval (tLetIn n b t) v -> *)
-  (*   exists b', *)
-  (*     eval b b' /\ eval (t {0 := b'}) v. *)
-  (* Proof. *)
-  (*   intros H; depind H; try solve_discr; try now easy. *)
-  (* Qed. *)
-
-  (* Lemma eval_Const {c v} : *)
-  (*   eval (tConst c) v -> *)
-  (*   exists decl body, declared_constant Σ c decl /\ *)
-  (*                     cst_body decl = Some body /\ *)
-  (*                     eval body v. *)
-  (* Proof. *)
-  (*   intros H; depind H; try solve_discr; try now easy. *)
-  (*   exists decl, body. intuition auto. *)
-  (* Qed. *)
-
-  (* Lemma eval_mkApps_tCoFix mfix idx l v : *)
-  (*   eval (mkApps (tCoFix mfix idx) l) v -> *)
-  (*   (exists l', Forall2 eval l l' /\ (v = mkApps (tCoFix mfix idx) l')). *)
-  (* Proof. *)
-  (*   intros H. *)
-  (*   depind H; try solve_discr. *)
-  (*   destruct (mkApps_elim a [t]). *)
-  (*   rewrite -[tApp _ _](mkApps_app f (firstn n l0) [t]) in x. *)
-  (*   solve_discr. *)
-  (*   specialize (IHeval1 _ _ _ eq_refl). *)
-  (*   firstorder eauto. *)
-  (*   solve_discr. *)
-  (*   destruct (mkApps_elim f [a]). *)
-  (*   rewrite -[tApp _ _](mkApps_app f (firstn n l0) [a]) in x. solve_discr. *)
-  (*   specialize (IHeval1 _ _ _ eq_refl). *)
-  (*   firstorder eauto. solve_discr. *)
-  (*   destruct (mkApps_elim f [arg]). *)
-  (*   rewrite -[tApp _ _](mkApps_app f (firstn n l0) [arg]) in x. solve_discr. *)
-  (*   specialize (IHeval1 _ _ _ eq_refl). destruct IHeval1. *)
-  (*   destruct H2. solve_discr. *)
-  (*   change (tApp f a) with (mkApps f [a]) in x. *)
-  (*   assert (l <> []). *)
-  (*   destruct l; simpl in *; discriminate. *)
-  (*   rewrite (app_removelast_last a H2) in x |- *. *)
-  (*   rewrite mkApps_app in x. simpl in x. inv x. *)
-  (*   specialize (IHeval1 _ _ _ eq_refl). *)
-  (*   destruct IHeval1 as [l' [evl' eqf']]. *)
-  (*   exists (l' ++ [a']). *)
-  (*   split. eapply Forall2_app; auto. constructor. now rewrite - !H5. constructor. *)
-  (*   subst f'. *)
-  (*   now rewrite mkApps_app. *)
-  (*   eapply atom_mkApps in H; intuition try easy. *)
-  (*   subst. *)
-  (*   exists []. intuition auto. *)
-  (* Qed. *)
-
-  (* Lemma eval_deterministic {t v v'} : eval t v -> eval t v' -> v = v'. *)
-  (* Proof. *)
-  (*   intros tv. revert v'. *)
-  (*   revert t v tv. *)
-  (*   induction 1 using eval_ind; intros v' tv'. *)
-  (*   - depelim tv'; auto. specialize (IHtv1 _ tv'1); congruence. *)
-  (*     specialize (IHtv1 _ tv'1). now subst. *)
-  (*     specialize (IHtv1 _ tv'1). now subst. easy. *)
-  (*   - depelim tv'; auto; try specialize (IHtv1 _ tv'1) || solve [depelim tv1]; try congruence. *)
-  (*     inv IHtv1. specialize (IHtv2 _ tv'2). subst. *)
-  (*     now specialize (IHtv3 _ tv'3). *)
-  (*     now subst f'. easy. *)
-  (*   - eapply eval_LetIn in tv' as [b' [evb evt]]. *)
-  (*     rewrite -(IHtv1 _ evb) in evt. *)
-  (*     eapply (IHtv2 _ evt). *)
-  (*   - depelim tv'; try solve_discr. *)
-  (*     * specialize (IHtv1 _ tv'1). *)
-  (*       solve_discr. inv H. *)
-  (*       now specialize (IHtv2 _ tv'2). *)
-  (*     * specialize (IHtv1 _ tv'1); solve_discr. *)
-  (*     * eapply eval_mkApps_tCoFix in tv1 as [l' [ev' eq]]. solve_discr. *)
-  (*     * easy. *)
-  (*   - subst. *)
-  (*     depelim tv'. *)
-  (*     * specialize (IHtv1 _ tv'1). *)
-  (*       solve_discr. *)
-  (*     * specialize (IHtv1 _ tv'1). *)
-  (*       now specialize (IHtv2 _ tv'2). *)
-  (*     * pose proof tv1. eapply eval_mkApps_tCoFix in H0. *)
-  (*       destruct H0 as [l' [evargs eq]]. solve_discr. *)
-  (*     * easy. *)
-  (*   - depelim tv' => //. *)
-  (*     * specialize (IHtv1 _ tv'1). discriminate. *)
-  (*     * specialize (IHtv1 _ tv'1). discriminate. *)
-  (*     * specialize (IHtv1 _ tv'1). inv IHtv1. *)
-  (*       rewrite H in H0. inv H0. *)
-  (*       now specialize (IHtv2 _ tv'2). *)
-  (*     * specialize (IHtv1 _ tv'1); subst. easy. *)
-
-  (*   - depelim tv'; try easy. *)
-  (*     * eapply eval_mkApps_tCoFix in tv'1 as [l' [evargs eq]]. *)
-  (*       solve_discr. *)
-  (*     * eapply eval_mkApps_tCoFix in tv'1 as [l' [evargs eq]]. *)
-  (*       solve_discr. *)
-  (*     * solve_discr. inv H1. rewrite H in H0. inv H0. *)
-  (*       now specialize (IHtv _ tv'). *)
-
-  (*   - depelim tv'; try easy. *)
-  (*     * solve_discr. inv H1. rewrite H in H0. inv H0. *)
-  (*       now specialize (IHtv _ tv'). *)
-  (*     * eapply eval_mkApps_tCoFix in tv'1 as [l' [evargs eq]]. *)
-  (*       solve_discr. *)
-  (*     * eapply eval_mkApps_tCoFix in tv' as [l' [evargs eq]]. *)
-  (*       solve_discr. *)
-
-  (*   - eapply eval_Const in tv' as [decl' [body' [? ?]]]. *)
-  (*     intuition eauto. eapply IHtv. *)
-  (*     red in isdecl, H0. rewrite H0 in isdecl. inv isdecl. *)
-  (*     now rewrite H in H2; inv H2. *)
-
-  (*   - depelim tv'. *)
-  (*     * eapply eval_mkApps_tCoFix in tv1 as [l' [evargs eq]]. *)
-  (*       solve_discr. *)
-  (*     * specialize (IHtv1 _ tv'1).  *)
-  (*       solve_discr. inv H. *)
-  (*       now specialize (IHtv2 _ tv'2). *)
-  (*     * specialize (IHtv1 _ tv'). solve_discr. *)
-  (*     * easy. *)
-
-  (*   - depelim tv'; try easy. *)
-  (*     * eapply eval_mkApps_tCoFix in tv as [l' [evargs eq]]. *)
-  (*       solve_discr. *)
-  (*     * specialize (IHtv _ tv'1). solve_discr. *)
-
-  (*   - depelim tv'; try specialize (IHtv1 _ tv'1); subst; try easy. *)
-  (*     specialize (IHtv2 _ tv'2). subst. reflexivity. *)
-
-  (*   - depelim tv'; try easy. *)
-  (* Qed. *)
-
-  (* Lemma eval_mkApps_cong f f' l l' : *)
-  (*   eval f f' -> *)
-  (*   value_head f' -> *)
-  (*   Forall2 eval l l' -> *)
-  (*   eval (mkApps f l) (mkApps f' l'). *)
-  (* Proof. *)
-  (*   revert l'. induction l using rev_ind; intros l' evf vf' evl. *)
-  (*   depelim evl. eapply evf. *)
-  (*   eapply Forall2_app_inv_l in evl as [? [? [? ?]]]. *)
-  (*   intuition auto. subst. depelim H1. depelim H1. *)
-  (*   rewrite !mkApps_app /=. eapply eval_app_cong; auto. *)
-  (*   destruct x0 using rev_ind; simpl; [|rewrite !mkApps_app]; simpl in *; destruct f'; *)
-  (*     try discriminate; constructor. *)
-  (* Qed. *)
+Lemma eval_deterministic {t v v'} :
+  eval t v ->
+  eval t v' ->
+  v = v'.
+Proof.
+  intros ev.
+  revert v'.
+  depind ev; intros v' ev'.
+  - depelim ev'.
+    + easy.
+    + now apply IHev1 in ev'1.
+    + apply IHev1 in ev'1; solve_discr.
+    + apply IHev1 in ev'1; solve_discr.
+    + apply IHev1 in ev'1; subst; easy.
+    + easy.
+  - depelim ev'.
+    + now apply IHev1 in ev'1.
+    + apply IHev1 in ev'1; subst.
+      apply IHev2 in ev'2; subst.
+      noconf ev'1.
+      now apply IHev3 in ev'3.
+    + apply IHev1 in ev'1; solve_discr.
+    + apply IHev1 in ev'1; solve_discr.
+    + apply IHev1 in ev'1; subst; easy.
+    + easy.
+  - depelim ev'.
+    + apply IHev1 in ev'1; subst.
+      now apply IHev2 in ev'2.
+    + easy.
+  - depelim ev'.
+    + apply IHev1 in ev'1; solve_discr.
+      noconf H.
+      now apply IHev2 in ev'2.
+    + apply IHev1 in ev'1; solve_discr.
+    + apply eval_mkApps_tCoFix in ev1 as (? & ?); solve_discr.
+    + easy.
+  - depelim ev'.
+    + apply IHev1 in ev'1; solve_discr.
+    + subst.
+      noconf H0.
+      now apply IHev2 in ev'2.
+    + apply eval_mkApps_tCoFix in ev1 as (? & ?); solve_discr.
+    + easy.
+  - depelim ev'.
+    + apply IHev1 in ev'1; solve_discr.
+    + apply IHev1 in ev'1; solve_discr.
+    + apply IHev1 in ev'1.
+      apply mkApps_eq_inj in ev'1; try easy.
+      depelim ev'1.
+      noconf H2.
+      subst.
+      apply IHev2 in ev'2; subst.
+      rewrite H4 in H.
+      now noconf H.
+    + apply IHev1 in ev'1.
+      apply mkApps_eq_inj in ev'1; try easy.
+      depelim ev'1.
+      noconf H2.
+      noconf H3.
+      apply IHev2 in ev'2.
+      subst.
+      rewrite H4 in H.
+      noconf H.
+      destruct H5 as [|(_ & ?)]; [easy|].
+      now apply negb_true_iff in H.
+    + apply IHev1 in ev'1.
+      subst.
+      rewrite isFixApp_mkApps in H2; [easy|].
+      cbn in *.
+      now rewrite orb_true_r in H2.
+    + easy.
+  - depelim ev'.
+    + apply IHev1 in ev'1; solve_discr.
+    + apply IHev1 in ev'1; solve_discr.
+    + apply IHev1 in ev'1.
+      apply IHev2 in ev'2.
+      apply mkApps_eq_inj in ev'1 as (ev'1 & <-); try easy.
+      noconf ev'1.
+      subst.
+      rewrite H1 in H.
+      noconf H.
+      destruct H0 as [|(? & ?)]; [easy|].
+      now apply negb_true_iff in H0.
+    + apply IHev1 in ev'1.
+      apply IHev2 in ev'2.
+      now apply mkApps_eq_inj in ev'1 as (ev'1 & <-).
+    + apply IHev1 in ev'1.
+      subst.
+      rewrite isFixApp_mkApps in H1; [easy|].
+      cbn in H1.
+      now rewrite orb_true_r in H1.
+    + easy.
+  - depelim ev'.
+    + apply eval_mkApps_tCoFix in ev'1 as (? & ?); solve_discr.
+    + apply eval_mkApps_tCoFix in ev'1 as (? & ?); solve_discr.
+    + apply mkApps_eq_inj in H1 as (H1 & <-); try easy.
+      noconf H1.
+      rewrite H0 in H.
+      noconf H.
+      now apply IHev in ev'.
+    + easy.
+  - depelim ev'.
+    + apply mkApps_eq_inj in H1 as (H1 & <-); try easy.
+      noconf H1.
+      rewrite H0 in H.
+      noconf H.
+      now apply IHev in ev'.
+    + apply eval_mkApps_tCoFix in ev'1 as (? & ?); solve_discr.
+    + apply eval_mkApps_tCoFix in ev' as (? & ?); solve_discr.
+    + easy.
+  - depelim ev'.
+    + unfold ETyping.declared_constant in *.
+      rewrite isdecl0 in isdecl.
+      noconf isdecl.
+      rewrite H0 in H.
+      noconf H.
+      now apply IHev in ev'.
+    + easy.
+  - depelim ev'.
+    + apply eval_mkApps_tCoFix in ev1 as (? & ?); solve_discr.
+    + apply IHev1 in ev'1.
+      now apply mkApps_eq_inj in ev'1 as (ev'1 & <-).
+    + apply IHev1 in ev'; solve_discr.
+    + easy.
+  - depelim ev'.
+    + apply eval_mkApps_tCoFix in ev as (? & ?); solve_discr.
+    + apply IHev in ev'1; solve_discr.
+    + easy.
+    + easy.
+  - depelim ev'.
+    + apply IHev1 in ev'1.
+      apply IHev2 in ev'2.
+      now subst.
+    + apply IHev1 in ev'1.
+      apply IHev2 in ev'2.
+      now subst.
+    + apply IHev1 in ev'1.
+      apply IHev2 in ev'2.
+      subst.
+      rewrite isFixApp_mkApps in H; [easy|].
+      cbn in H.
+      now rewrite orb_true_r in H.
+    + apply IHev1 in ev'1.
+      apply IHev2 in ev'2.
+      now subst.
+    + apply IHev1 in ev'1.
+      apply IHev2 in ev'2.
+      congruence.
+    + easy.
+  - now depelim ev'.
+Qed.
 
 End Wcbv.
